cla/Cla/ParseDefs.lean
@@ -1,0 +1,18 @@
+import Cla.Com
+
+
+
+namespace Cla
+
+
+
+def Parse.flagArgs
+  (argSpec : ArgSpec σ)
+: IParseM (EStateM String σ Unit) :=
+  ArgSpec.Bounds.MProdRun
+    argSpec.bounds
+    Parse.nextFlagArg
+    (Parse.flagAllArgs argSpec.bounds.max)
+    argSpec.validator
+
+
