cla/Main.lean
@@ -1,4 +1,7 @@
 import Cla
 
-def main : IO Unit :=
-  IO.println s!"lif sux"
+def main (args : List String) : IO Unit :=
+  do
+    IO.println s!"lif sux"
+    for arg in args do
+      IO.println s!"arg : {arg}"
